common/SmallstepMulti.v
@@ -13,30 +13,41 @@ Require Import Values Maps Memory AST.
 Module NatIndexed.
     Definition t := nat.
 
-    Fixpoint index (n : nat) : positive :=
+    Definition index (n : nat) : positive :=
       match n with
       |O => 1%positive
-      |S n => 1 + index n
+      |_ => 1 + Pos.of_nat n
       end.
 
-    (*wrong, fix it later*)
     Definition index_rev (p:positive) : nat :=
-      Pos.to_nat p.
+      match p with
+      |xH => O
+      |_ => Pos.to_nat p -1
+    end.
 
     Lemma t_positive_t : forall (n:nat), index_rev (index n) = n.
-    Admitted.
+    Proof.
+      intros.
+      destruct (index n) eqn:Hn; unfold index_rev; destruct n; unfold index in *; lia.
+    Qed.
 
     Lemma positive_t_positive : forall (p:positive), index(index_rev p) = p.
-    Admitted.
+    Proof.
+      intros. destruct (index_rev p) eqn:Hp; unfold index; destruct p; unfold index_rev in *; lia.
+    Qed.
 
     Lemma index_inj : forall (x y : nat), index x = index y -> x = y.
-    Admitted.
-
+    Proof.
+      destruct x; destruct y; unfold index in *; lia.
+    Qed.
+    
     Definition eq := Nat.eq_dec.
 End NatIndexed.
 
 Module NatMap := IRMap(NatIndexed).
-    
+
+(** Unchecked concern: Do we need to define new events for [yield] and [pthread_create] ? Can we keep the internal events?
+    Now this two points are implemented differernt with CASCompCert *)
 Section MultiThread.
 
   Context {OpenS : semantics li_c li_c}.
@@ -55,24 +66,21 @@ Section MultiThread.
   
   Definition OpenLTS := activate OpenS initial_se.
   Definition ClosedS := Closed.close_semantics initial_query final_reply OpenS initial_se.
-  
-  (* The global state of concurrent semantics *)
 
-  (* problem : how to deal with "thread variable" *)
-
-  (* Definition state := list local_state. *)
-
-
+  (* We need an interface to get and set global memory from local_state *)
+  (* Not sure if this is proper, maybe need some lemmas about these operations *)
   Variable get_gmem : local_state -> mem.
   Variable set_gmem : mem -> local_state -> local_state.
 
+  (*
   Definition tid_mem (m:mem) : nat :=
     Mem.tid (Mem.support m).
 
   Definition stacks_mem (m:mem) :=
     Mem.stacks (Mem.support m).
-
-  (* Definition and operations of global state *)
+   *)
+  
+  (** * Definition and operations of global state *)
 
     Record state : Type := mk_gstate
     {
@@ -87,30 +95,51 @@ Section MultiThread.
     }.
 
   Definition empty_threads : NatMap.t (option local_state) := NatMap.init None.
-  (* Definition initial_threads (ls :local_state) := NatMap.set 1%nat (Some ls) empty_threads.
-  Program Definition single_state (ls: local_state) := mk_gstate (initial_threads ls) 1%nat 2%nat false. *)
-
   
-  Definition update_threads (s : state) (t: NatMap.t (option local_state)) :=
+  Definition update_threads (s: state) (t: NatMap.t (option local_state)) :=
     mk_gstate t (cur_tid s) (next_tid s) .
 
+  Definition update_thread (s: state) (tid : nat) (ls: local_state) :=
+    mk_gstate (NatMap.set tid (Some ls) (threads s)) (cur_tid s) (next_tid s).
+
+  Definition update_cur_thread (s: state) (ls : local_state) := update_thread s (cur_tid s) ls.
+  
+  Definition get_thread (s: state) (tid: nat) :=
+    NatMap.get tid (threads s).
+
+  Definition get_cur_thread (s: state) := get_thread s (cur_tid s).
+  
+  Definition update_cur_tid (s: state) (tid : nat) :=
+    mk_gstate (threads s) tid (next_tid s).
+
+  Definition update_next_tid (s: state) (tid: nat) :=
+    mk_gstate (threads s) (cur_tid s) tid.
+  
   Variable yield_strategy : state -> nat.
   Axiom yield_strategy_range : forall s, (1 < yield_strategy s < (next_tid s))%nat.
   (*some other properties may be added here, such as only point to active threads *)
 
-  (* We transfer to thread tid' and update its local_state to ls (synchronize the global memory for it) *)
-  Definition yield_state (s : state) (ls : local_state): state :=
-    match s with
-      mk_gstate threads cid nid =>
-        let tid' := yield_strategy s in
-        let threads' := NatMap.set tid' (Some ls) threads in
-      mk_gstate threads' tid' nid
+  (* We transfer to thread tid' and update
+     its local_state with an updated memory *)
+
+  Definition yield_state (s: state) (gmem: mem): state :=
+    let tid' := yield_strategy s in
+    let s' := update_cur_tid s tid' in
+    match get_cur_thread s with (*yield_strategy and the inv should guarantee we get Some here*)
+    |Some ls => update_thread s' tid' (set_gmem gmem ls)
+    |None => s'
     end.
 
-  
-  (* problem here, we need some proofs about initial local_state for this initial gstate
-   *)
-
+  (* We add a new thread with its initial local state, we also update the running memory by adding a new list of positives *)
+  Definition pthread_create_state (s: state) (ls : local_state) (gmem : mem): state :=
+    let ntid := (next_tid s) in let ctid := (cur_tid s) in
+    let s' := update_next_tid s (S ntid) in
+    let s'' := update_thread s' ntid ls in
+    match get_cur_thread s with
+    |Some ls => update_thread s'' ctid (set_gmem gmem ls)
+    |None => s'
+    end.
+    
   Definition genvtype := Smallstep.genvtype OpenLTS.
   
   (** Initial state of Concurrent semantics *)
@@ -121,7 +150,7 @@ Section MultiThread.
   Inductive initial_state : state -> Prop :=
   |initial_state_intro : forall ls s,
       cur_tid s = 1%nat -> next_tid s = 2%nat ->
-      NatMap.get 1%nat (threads s) = Some ls ->
+      get_cur_thread s = Some ls ->
       (Closed.initial_state ClosedS) ls ->
       initial_state s.
 
@@ -129,49 +158,72 @@ Section MultiThread.
   Inductive final_state : state -> int -> Prop :=  
   |final_state_intro : forall ls i s,
       cur_tid s = 1%nat ->
-      NatMap.get 1%nat (threads s) = Some ls ->
+      get_cur_thread s = Some ls ->
+      (Closed.final_state ClosedS) ls i->
       final_state s i.
+
+  (** * Definitions about the primitive yield *)
 
   Definition yield_id := 1001%positive.
   Definition yield_sig := mksignature nil Tvoid cc_default.
+
+  (* Definition func_yield_external : fundef :=
+    External (EF_external "yield" yield_sig).  *)
   
   Inductive query_is_yield : query li_c -> Prop :=
   |yield_intro : forall b m,
     Genv.find_symbol initial_se yield_id = Some b ->
     query_is_yield (cq (Vptr b Ptrofs.zero) yield_sig nil m).
+
+  (** * Definitions about the primitive pthread_create *)
+
+  Definition pthread_create_id := 1002%positive.
+  
+  (* int pthread_create (void * (*start_routine) (void*), void* arg) *)
+  (* TODO: not quite sure to use Tlong or Tany64 here, we used Tlong for function pointer in the Client-Server example *)
+  Definition pthread_create_sig := mksignature (Tlong :: Tlong :: nil) Tint cc_default.
+
+  
+  (** Problem here: the type of start_routine here may not be accecpted by [initial_state] in Clight semantics. *)
+  (** Maybe we have to do sth more to support such void* (*f) (void*) prototype, maybe not using cc_default *)
+  Definition start_routine_sig := mksignature (Tlong :: nil) Tlong cc_default.
+
+
+  (* turns a call to pthread_create into a call to the start_routine, the initial memory is updated in 2nd query *)
+  Inductive query_is_pthread_create : query li_c -> query li_c -> Prop :=
+  |pthread_create_intro :
+    forall m arglist b_ptc b_start b_arg ofs m'
+      (FINDPTC: Genv.find_symbol initial_se pthread_create_id = Some b_ptc)
+      (ARGLIST: arglist = (Vptr b_start Ptrofs.zero) :: (Vptr b_arg ofs) :: nil)
+      (MEM_CREATE: Mem.thread_create m = m'),
+      query_is_pthread_create
+        (cq (Vptr b_ptc Ptrofs.zero) pthread_create_sig arglist m)
+        (cq (Vptr b_start Ptrofs.zero) start_routine_sig ((Vptr b_arg ofs)::nil) m').
+
   
   Inductive step : genvtype -> state -> trace -> state -> Prop :=
-  |step_local : forall ge ls1 t ls2 tid s s' threads',
-      let threads := threads s in
-      NatMap.get tid threads = Some ls1 ->
+  |step_local : forall ge ls1 t ls2 s s',
+      get_cur_thread s = Some ls1 ->
       Smallstep.step OpenLTS ge ls1 t ls2 ->
-      threads' = NatMap.set tid (Some ls2) threads ->
-      s' = update_threads s threads ->
+      update_thread s (cur_tid s) ls2 = s' ->
       step ge s t s'
-  |step_thread_yield : forall ge s tid s' tid' gmem ls ls1 ls1' q,
-      NatMap.get tid (threads s) = Some ls ->
-      at_external OpenLTS ls q ->
+  |step_thread_yield : forall ge s s' tid' ls q gmem' p,
+      get_cur_thread s = Some ls ->
+      Smallstep.at_external OpenLTS ls q ->
       query_is_yield q ->
-      cq_mem q = gmem ->
-      NatMap.get tid' (threads s) = Some ls1 ->
-      set_gmem gmem ls1 = ls1' ->
-      yield_strategy s = tid' ->      
-      yield_state s ls1' = s' ->
+      yield_strategy s = tid' ->
+      (*the proof p may be a problem, provided from the invariant between state and the support in gmem *)
+      Mem.yield (cq_mem q) tid' p = gmem' -> 
+      yield_state s gmem' = s' ->
+      step ge s E0 s'
+  |step_thread_create : forall ge s s' q_ptc q_str new_ls gmem ls,
+      get_cur_thread s = Some ls ->
+      Smallstep.at_external OpenLTS ls q_ptc ->
+      query_is_pthread_create q_ptc q_str ->
+      Smallstep.initial_state OpenLTS q_str new_ls ->
+      cq_mem q_str = gmem -> (* The global memory is already updated from q_ptc to q_str *)
+      pthread_create_state s new_ls gmem = s' ->
       step ge s E0 s'.
-  |step_thread_create : ge s tid s' q,
-      NatMap.get tid (threads s) = Some ls ->
-      at_external OpenLTS ls q ->
-      query_is_create q ->
-      
-      
-      step ge s E0 s'.
-           
-      
-  (* problem : how to simultaneously update the memory for all threads *)
-  |Step_lock
-  |Step_unlock
-  |Step_thread_create
-     
-  |Step_thread_join
-   
+  
+End MultiThread.   
   
