common/Smallstep.v
@@ -545,16 +545,17 @@ Record lts liA liB state: Type := {
 Record semantics liA liB := {
   skel: AST.program unit unit;
   state: Type;
-  memory_of_state : state -> mem;
+  (* get_mem : state -> mem;
+  set_mem : state -> mem -> state; *)
   activate :> Genv.symtbl -> lts liA liB state;
 }.
 
 (** Handy notations. *)
 
-Notation Semantics_gen memory_of_state step initial_state at_ext after_ext final_state globalenv p :=
+Notation Semantics_gen (* memory_of_state *) step initial_state at_ext after_ext final_state globalenv p :=
   {|
     skel := AST.erase_program p;
-    memory_of_state := memory_of_state;
+    (* memory_of_state := memory_of_state; *)
     activate se :=
       let ge := globalenv se p in
       {|
@@ -568,8 +569,8 @@ Notation Semantics_gen memory_of_state step initial_state at_ext after_ext final
       |};
   |}.
 
-Notation Semantics memory_of_state step initial_state at_ext after_ext final_state p :=
-  (Semantics_gen memory_of_state step initial_state at_ext (fun _ => after_ext) (fun _ => final_state) (@Genv.globalenv _ _) p).
+Notation Semantics (* memory_of_state *) step initial_state at_ext after_ext final_state p :=
+  (Semantics_gen (* memory_of_state *) step initial_state at_ext (fun _ => after_ext) (fun _ => final_state) (@Genv.globalenv _ _) p).
 
 Declare Scope smallstep_scope.
 
@@ -2338,7 +2339,7 @@ Definition atomic : semantics liA liB :=
 {|
   skel := skel L;
   state := trace * state L;
-  memory_of_state := fun s => (memory_of_state L) (snd s);
+  (* memory_of_state := fun s => (memory_of_state L) (snd s); *)
   activate se := {|
     genvtype := genvtype (L se);
     step := atomic_step se;
