common/SmallstepLinking.v
@@ -71,11 +71,11 @@ Section LINK.
     Definition valid_query q :=
       valid_query (L true se) q || valid_query (L false se) q.
 
-    Definition memory_of_state (s: state) : mem :=
+    (* Definition memory_of_state (s: state) : mem :=
       match s with
       |nil => Mem.empty
       |(st i ss) :: _ => (memory_of_state (L i)) ss
-      end.
+      end. *)
     
   End WITH_SE.
 
@@ -83,7 +83,7 @@ Section LINK.
 
   Definition semantics: semantics li li :=
     {|
-      Smallstep.memory_of_state := memory_of_state;
+      (* Smallstep.memory_of_state := memory_of_state; *)
       activate se :=
         {|
           Smallstep.step ge := step se;
